SepLogic_Misc.thy
@@ -1,0 +1,167 @@
+theory SepLogic_Misc
+imports "../Imperative_HOL_Time/SepLogicTime/SepAuto"
+begin
+
+
+lemma mod_star_trueI: "h\<Turnstile>P \<Longrightarrow> h\<Turnstile>P*true"  
+  by (metis assn_times_comm entailsD' entails_true mult.left_neutral) 
+
+
+lemma merge_true_star[simp]: "true*true = true"
+  using top_assn_reduce by auto
+
+lemma mod_false[simp]: "\<not> h\<Turnstile>false"  
+  by (simp add: pure_assn_rule)
+lemma mod_pure_star_dist[simp]: "h\<Turnstile>P*\<up>b \<longleftrightarrow> h\<Turnstile>P \<and> b"
+  by (simp add: mod_pure_star_dist)
+
+
+lemma pure_assn_eq_conv[simp]: "\<up>P = \<up>Q \<longleftrightarrow> P=Q" 
+  by (metis (full_types) assn_times_comm empty_iff in_range.simps mod_false' mod_pure_star_dist top_assn_rule)
+
+thm entailsD
+
+lemma ent_true[simp]: "P \<Longrightarrow>\<^sub>A true" 
+  by (simp add: entails_true) 
+
+
+
+lemma ent_star_mono: "\<lbrakk> P \<Longrightarrow>\<^sub>A P'; Q \<Longrightarrow>\<^sub>A Q'\<rbrakk> \<Longrightarrow> P*Q \<Longrightarrow>\<^sub>A P'*Q'" 
+  using entail_trans2 entails_frame by blast
+
+
+lemma merge_true_star_ctx: "true * (true * P) = true * P"
+  by (metis assn_times_assoc top_assn_reduce)
+
+lemma pf: "(a::assn) * b = b * a" 
+  using assn_times_comm by auto 
+
+lemma ent_true_drop: 
+  "P\<Longrightarrow>\<^sub>AQ*true \<Longrightarrow> P*R\<Longrightarrow>\<^sub>AQ*true"
+  "P\<Longrightarrow>\<^sub>AQ \<Longrightarrow> P\<Longrightarrow>\<^sub>AQ*true"
+  apply (metis assn_times_comm ent_star_mono ent_true merge_true_star_ctx)
+  apply (metis assn_one_left ent_star_mono ent_true pf)
+  done
+
+
+
+
+lemma entailsI: 
+  assumes "\<And>h. h\<Turnstile>P \<Longrightarrow> h\<Turnstile>Q"
+  shows "P \<Longrightarrow>\<^sub>A Q" 
+  using assms unfolding entails_def by auto
+
+lemma entt_refl': "P\<Longrightarrow>\<^sub>A P * true" 
+  by (simp add: entailsI mod_star_trueI) 
+
+subsection "for relH"
+
+text "Transitivity"
+lemma relH_trans[trans]: "\<lbrakk>relH as h1 h2; relH as h2 h3\<rbrakk> \<Longrightarrow> relH as h1 h3"
+  unfolding relH_def
+  by auto
+
+lemma in_range_subset: 
+  "\<lbrakk>as \<subseteq> as'; in_range (h,as')\<rbrakk> \<Longrightarrow> in_range (h,as)"
+  by (auto simp: in_range.simps)
+
+lemma relH_subset:
+  assumes "relH bs h h'"
+  assumes "as \<subseteq> bs"
+  shows "relH as h h'"
+  using assms unfolding relH_def by (auto intro: in_range_subset)
+
+subsection "new_addrs"
+
+lemma new_addrs_id[simp]: "(new_addrs h as h) = as" unfolding new_addrs_def by auto
+
+subsection "entailst"
+
+definition entailst :: "assn \<Rightarrow> assn \<Rightarrow> bool" (infix "\<Longrightarrow>\<^sub>t" 10)
+  where "entailst A B \<equiv> A \<Longrightarrow>\<^sub>A B * true"
+lemma enttI: "A\<Longrightarrow>\<^sub>AB*true \<Longrightarrow> A\<Longrightarrow>\<^sub>tB" unfolding entailst_def .
+lemma enttD: "A\<Longrightarrow>\<^sub>tB \<Longrightarrow> A\<Longrightarrow>\<^sub>AB*true" unfolding entailst_def .
+                                   
+lemma ent_trans[trans]: "\<lbrakk> P \<Longrightarrow>\<^sub>A Q; Q \<Longrightarrow>\<^sub>AR \<rbrakk> \<Longrightarrow> P \<Longrightarrow>\<^sub>A R"
+  by (auto intro: entailsI dest: entailsD)
+
+
+lemma entt_trans:
+  "entailst A B \<Longrightarrow> entailst B C \<Longrightarrow> entailst A C"
+  unfolding entailst_def
+  apply (erule ent_trans)
+  by (metis assn_times_assoc ent_star_mono ent_true merge_true_star)  
+
+lemma ent_imp_entt: "P\<Longrightarrow>\<^sub>AQ \<Longrightarrow> P\<Longrightarrow>\<^sub>tQ" 
+  apply (rule enttI)
+  apply (erule ent_trans)
+  by (simp add: entailsI mod_star_trueI)  
+
+
+lemma entt_refl: "P\<Longrightarrow>\<^sub>t P " 
+  by (simp add: entailst_def entailsI mod_star_trueI) 
+
+subsection "Heap Or"
+
+
+definition hor :: "assn \<Rightarrow> assn \<Rightarrow> assn" (infixr "\<or>\<^sub>A" 61)  where "hor A B = Abs_assn (Assn (
+    \<lambda>h. h\<Turnstile>A \<or> h\<Turnstile>B ) )"
+
+
+
+lemma ent_disjI1_direct[simp]: "A \<Longrightarrow>\<^sub>A A \<or>\<^sub>A B"
+  sorry
+
+lemma ent_disjI2_direct[simp]: "B \<Longrightarrow>\<^sub>A A \<or>\<^sub>A B"
+  sorry
+
+lemma entt_disjI1_direct[simp]: "A \<Longrightarrow>\<^sub>t A \<or>\<^sub>A B"
+  by (rule ent_imp_entt[OF ent_disjI1_direct])
+
+lemma entt_disjI2_direct[simp]: "B \<Longrightarrow>\<^sub>t A \<or>\<^sub>A B"
+  by (rule ent_imp_entt[OF ent_disjI2_direct])
+
+lemma ent_disjE: "\<lbrakk> A\<Longrightarrow>\<^sub>AC; B\<Longrightarrow>\<^sub>AC \<rbrakk> \<Longrightarrow> A\<or>\<^sub>AB \<Longrightarrow>\<^sub>AC"
+  unfolding entails_def sorry
+
+
+
+subsection \<open>New command ureturn\<close>
+
+definition ureturn :: "'a \<Rightarrow> 'a Heap" where
+  [code del]: "ureturn x = Heap_Monad.heap (\<lambda>h. (x,h,0))"
+
+lemma execute_ureturn [execute_simps]:
+  "execute (ureturn x) = Some \<circ> (\<lambda>h. (x,h,0))"
+  by (simp add: ureturn_def execute_simps)
+
+lemma success_ureturnI [success_intros]:
+  "success (ureturn x) h"
+  by (rule successI) (simp add: execute_simps)
+
+lemma effect_ureturnI [effect_intros]:
+  "h = h' \<Longrightarrow> effect (ureturn x) h h' x 0"
+  by (rule effectI) (simp add: execute_simps)
+
+lemma effect_ureturnE [effect_elims]:
+  assumes "effect (ureturn x) h h' r n"
+  obtains "r = x" "h' = h" "n=0"
+  using assms by (rule effectE) (simp add: execute_simps)
+thm execute_return'
+
+lemma execute_ureturn' [rewrite]: "execute (ureturn x) h = Some (x, h, 0)" by (metis comp_eq_dest_lhs execute_ureturn)
+
+lemma run_ureturnD: "run (ureturn x) (Some h) \<sigma> r t \<Longrightarrow> \<sigma> = Some h \<and> r = x \<and> t = 0"
+  by (auto simp add: execute_ureturn' run.simps)
+
+lemma return_rule:
+  "<$0> ureturn x <\<lambda>r. \<up>(r = x)>" 
+  unfolding hoare_triple_def apply (auto dest!: run_ureturnD simp: timeCredit_assn_rule)
+  subgoal by (metis (mono_tags, hide_lams) pheap.sel(2) pheap.sel(3) pure_assn_rule)
+  subgoal using relH_def by fastforce 
+  done
+
+
+
+
+end
